**#2** \
**a)** xyz + x(yz)′ + x′(y + z) + (xyz)′ = \
xyz + (xyz)' + x(yz)'+ x'(y + z) = \
1 + x(yz)' + x'(y + z) = 1 \
X | Y | Z | F \
0 | 0 | 0 | 1 \
0 | 0 | 1 | 1 \
0 | 1 | 0 | 1 \
0 | 1 | 1 | 1 \
1 | 0 | 0 | 1 \
1 | 0 | 1 | 1 \
1 | 1 | 0 | 1 \
1 | 1 | 1 | 1 \
**b)** (x + y′)(x′ + z′)(y′ + z′) = \
(x + y′)(x′ + z′)(y' + z' + x)(y' + z' + x') = \
(x' + y')(x' + z') \
A = x + y' \
B = x' + z' \
F = (x' + y')(x' + z') \
X | Y | Z | A | B | F | \
0 | 0 | 0 | 1 | 1 | 1 | \
0 | 0 | 1 | 1 | 1 | 1 | \
0 | 1 | 0 | 0 | 1 | 0 | \
0 | 1 | 1 | 0 | 1 | 0 | \
1 | 0 | 0 | 1 | 1 | 1 | \
1 | 0 | 1 | 1 | 0 | 0 | \
1 | 1 | 0 | 1 | 1 | 1 | \
1 | 1 | 1 | 1 | 0 | 0 | \
**#4** \
F if F(x,y,z) = (x′ + y)(x + z)(y′ + z)′ = \
[(~~x~~ + y)(x + z)~~(~~y~~ + z)~~] ' \
{~~AB~~ = ~~A~~ + B } \
{~~A + B~~ = ~~A~~ * ~~B~~}
